Main.lean
@@ -2,6 +2,6 @@ import ParserCombinators
 
 def main (args : List String) : IO UInt32 := match args with
   | [s] => do
-    IO.println $ (runParser'.{0} (μ := Option) concatParser s).1.toList
+    IO.println $ (runParser'.{0} (μ := Const) concatParser s).1.toList
     pure 0
   | _ => pure 1
