ParserCombinators.lean
@@ -3,5 +3,5 @@
 import ParserCombinators.Basic
 import ParserCombinators.Memoized
 import ParserCombinators.CFG
-import ParserCombinators.Example
+-- import ParserCombinators.Example
 import ParserCombinators.Example2
